src/QUIC.Impl.Base.fst
@@ -1,0 +1,118 @@
+module QUIC.Impl.Base
+open QUIC.Spec.Base
+
+module B = LowStar.Buffer
+module U8 = FStar.UInt8
+module U64 = FStar.UInt64
+module U32 = FStar.UInt32
+module Spec = QUIC.Spec.Base
+
+/// Information stored in a QUIC header. This is a Low* type passed by value --
+/// it's a little expensive. Consider passing it by reference in ``encrypt``?
+///
+/// Note that we try to follow the convention of buffer arguments followed by
+/// their lengths.
+
+noeq type long_header_specifics =
+  | BInitial:
+    payload_length: uint62_t ->
+    packet_number: uint62_t ->
+    packet_number_length: packet_number_length_t ->
+    token: B.buffer U8.t -> (* I reordered those so that the extracted code for this type is a tagged union with common prefixes *)
+    token_length: U32.t { let v = U32.v token_length in v == B.length token /\ 0 <= v /\ v <= token_max_len  } ->
+    long_header_specifics
+  | BZeroRTT:
+    payload_length: uint62_t ->
+    packet_number: uint62_t ->
+    packet_number_length: packet_number_length_t ->
+    long_header_specifics
+  | BHandshake:
+    payload_length: uint62_t ->
+    packet_number: uint62_t ->
+    packet_number_length: packet_number_length_t ->
+    long_header_specifics
+  | BRetry:
+    unused: bitfield 4 ->
+    odcid: B.buffer U8.t ->
+    odcil: U32.t { let v = U32.v odcil in v = B.length odcid /\ 0 <= v /\ v <= 20 } ->
+    long_header_specifics
+
+noeq type header =
+  | BLong:
+    version: U32.t ->
+    dcid: B.buffer U8.t ->
+    dcil: U8.t { let v = U8.v dcil in v == B.length dcid /\ 0 <= v /\ v <= 20 } ->
+    scid: B.buffer U8.t ->
+    scil: U8.t { let v = U8.v scil in v == B.length scid /\ 0 <= v /\ v <= 20 } ->
+    spec: long_header_specifics ->
+    header
+  | BShort:
+    spin: bool ->
+    phase: bool ->
+    cid: B.buffer U8.t ->
+    cid_len: U8.t{
+      let l = U8.v cid_len in
+      U8.v cid_len == B.length cid /\
+      0 <= U8.v cid_len /\ U8.v cid_len <= 20
+    } ->
+    packet_number: uint62_t ->
+    packet_number_length: packet_number_length_t ->
+    header
+
+module HS = FStar.HyperStack
+
+let header_live (h: header) (m: HS.mem) : GTot Type0 =
+  match h with
+  | BShort spin phase cid cid_len packet_number packet_number_length ->
+    B.live m cid
+  | BLong version dcid dcil scid scil spec ->
+    B.live m dcid /\ B.live m scid /\
+    begin match spec with
+    | BInitial payload_length packet_number packet_number_length token token_length ->
+      B.live m token
+    | BRetry unused odcid odcil ->
+      B.live m odcid
+    | _ -> True
+    end
+
+let header_footprint (h: header) : GTot B.loc =
+  match h with
+  | BShort spin phase cid cid_len packet_number packet_number_length ->
+    B.loc_buffer cid
+  | BLong version dcid dcil scid scil spec ->
+    (B.loc_buffer dcid `B.loc_union` B.loc_buffer scid) `B.loc_union`
+    begin match spec with
+    | BInitial payload_length packet_number packet_number_length token token_length ->
+      B.loc_buffer token
+    | BRetry unused odcid odcil ->
+      B.loc_buffer odcid
+    | _ -> B.loc_none
+    end
+
+module FB = FStar.Bytes
+
+let g_header (h: header) (m: HS.mem) : GTot Spec.header =
+  match h with
+  | BShort spin phase cid cid_len packet_number packet_number_length ->
+    MShort spin phase (FB.hide (B.as_seq m cid)) packet_number_length packet_number
+  | BLong version dcid dcil scid scil spec ->
+    MLong version (FB.hide (B.as_seq m dcid)) (FB.hide (B.as_seq m scid))
+      begin match spec with
+      | BInitial payload_length packet_number packet_number_length token token_length ->
+        MInitial (FB.hide (B.as_seq m token)) payload_length packet_number_length packet_number
+      | BZeroRTT payload_length packet_number packet_number_length ->
+        MZeroRTT payload_length packet_number_length packet_number
+      | BHandshake payload_length packet_number packet_number_length ->
+        MHandshake payload_length packet_number_length packet_number
+      | BRetry unused odcid odcil ->
+        MRetry unused (FB.hide (B.as_seq m odcid))
+      end
+
+let frame_header
+  (h: header)
+  (l: B.loc)
+  (m1 m2: HS.mem)
+: Lemma
+  (requires (header_live h m1 /\ B.modifies l m1 m2 /\ B.loc_disjoint l (header_footprint h)))
+  (ensures (header_live h m2 /\ g_header h m2 == g_header h m1))
+= ()
